abstractified vector Tried to directly axiomatize the index based memory operations on vectors and prevent direct reading and writing of vectors. Perhaps the Ghost effect will help

examples/low-level/mvector.fsi
@@ -1,0 +1,43 @@
+(*--build-config
+    options:--admit_fsi Set --z3timeout 10;
+    variables:LIB=../../lib;
+    other-files:$LIB/ext.fst $LIB/set.fsi $LIB/heap.fst $LIB/st.fst $LIB/list.fst  stack.fst listset.fst st3.fst $LIB/constr.fst word.fst
+  --*)
+
+module MVector
+open StructuredMem
+open MachineWord
+
+(*
+    Can we generalize vector to cover all the algebraic types definable in C?
+*)
+type vector : Type -> nat -> Type
+
+(*can we make them ghosts*)
+val updateIndex : #a:Type -> #n:nat -> (vector a n)
+  -> index:nat{index<n} -> a -> Tot (vector a n)
+
+val atIndex : #a:Type -> #n:nat -> (vector a n)
+  -> index:nat{index<n} -> Tot a
+
+
+val readIndex :  #a:Type -> #n:nat -> r:(ref (vector a n))
+  -> index:nat{index<n} -> PureMem a (fun m -> b2t (refExistsInMem r m)) (fun _ _ _-> True)
+
+
+val updIndex :  #a:Type -> #n:nat -> r:(ref (vector a n))
+  -> index:(index:nat{index<n}) -> newV:a ->
+ Mem unit
+    (requires (fun m -> b2t (refExistsInMem r m)))
+    (ensures (fun m0 _ m1-> (refExistsInMem r m0) /\ m1= (writeMemAux r  m0 (updateIndex (loopkupRef r m0) index newV))))
+
+(*There is no way to read or write a whole vector.
+
+(Technically, you can read a vector, but there's nothing you can do with
+  the result if updateIndex and atIndex are ghosts.)
+
+This seems closer to C's lvalue/rvalue semantics.
+
+If we allowed a program to read
+ a full vector and apply some blackbox/convoluted function to it,
+ and write it back, what would the compiler do?*)
