examples/low-level/mvector.fst
@@ -1,0 +1,37 @@
+(*--build-config
+    options:--admit_fsi Set --z3timeout 10;
+    variables:LIB=../../lib;
+    other-files:$LIB/ext.fst $LIB/set.fsi $LIB/heap.fst $LIB/st.fst $LIB/list.fst  stack.fst listset.fst st3.fst $LIB/constr.fst word.fst mvector.fsi
+  --*)
+
+module MVector
+open StructuredMem
+open MachineWord
+open Seq
+
+type vector (a:Type) (n:nat) = (index:nat{index<n} -> Tot a)
+
+let updateIndex 'a #n f index newV =
+  (fun indx -> if (indx= index) then newV else f indx)
+
+let atIndex 'a #n f index  =
+   f index
+
+(* When F* complains that effect ALL and StSTATE cannot be combined,
+  see whether you missed a Tot somewhere.
+  Is there a way to make Tot the default effect, instead of ALL
+*)
+
+(*val readIndex :  #a:Type -> #n:nat -> r:(ref (vector a n))
+  -> index:nat{index<n} -> Mem a (fun m -> b2t (refExistsInMem r m)) (fun _ _ _-> True)*)
+let readIndex 'a #n r index =
+  let rv = (memread r) in (atIndex rv index)
+
+(*Can one reinclude the types from the FSI file?*)
+
+(*val updIndex :  #a:Type -> #n:nat -> r:(ref (vector a n))
+  -> index:nat{index<n} -> a ->
+ Mem unit (fun m -> b2t (refExistsInMem r m)) (fun _ _ _-> True)*)
+let updIndex 'a #n r index newV =
+  let rv = (memread r) in
+  memwrite r (updateIndex rv index newV)
